push opaque ops through TaggedComp

src/HigherValue.v
@@ -1,11 +1,15 @@
 Require Import oeuf.Common.
 Require Import oeuf.Metadata.
+Require Import oeuf.OpaqueTypes.
+Require Import StructTact.StructTactics.
+Require Import oeuf.EricTact.
 
 Definition function_name := nat.
 
 Inductive value :=
 | Constr (tag : nat) (args : list value)
 | Close (f : function_name) (free : list value)
+| Opaque (ty : opaque_type_name) (v : opaque_type_denote ty)
 .
 
 Definition value_rect_mut
@@ -13,6 +17,7 @@ Definition value_rect_mut
         (Pl : list value -> Type)
     (HConstr :  forall tag args, Pl args -> P (Constr tag args))
     (HClose :   forall fname free, Pl free -> P (Close fname free))
+    (HOpaque :  forall ty v, P (Opaque ty v))
     (Hnil :     Pl [])
     (Hcons :    forall v vs, P v -> Pl vs -> Pl (v :: vs))
     (v : value) : P v :=
@@ -25,6 +30,7 @@ Definition value_rect_mut
         match v as v_ return P v_ with
         | Constr tag args => HConstr tag args (go_list args)
         | Close fname free => HClose fname free (go_list free)
+        | Opaque ty v => HOpaque ty v
         end in go v.
 
 Definition value_rect_mut'
@@ -32,6 +38,7 @@ Definition value_rect_mut'
         (Pl : list value -> Type)
     (HConstr :  forall tag args, Pl args -> P (Constr tag args))
     (HClose :   forall fname free, Pl free -> P (Close fname free))
+    (HOpaque :  forall ty v, P (Opaque ty v))
     (Hnil :     Pl [])
     (Hcons :    forall v vs, P v -> Pl vs -> Pl (v :: vs)) :
     (forall v, P v) * (forall vs, Pl vs) :=
@@ -44,6 +51,7 @@ Definition value_rect_mut'
         match v as v_ return P v_ with
         | Constr tag args => HConstr tag args (go_list args)
         | Close fname free => HClose fname free (go_list free)
+        | Opaque ty v => HOpaque ty v
         end in
     let fix go_list vs :=
         match vs as vs_ return Pl vs_ with
@@ -62,9 +70,10 @@ Tactic Notation "multi_induction" constr(x) "using" uconstr(scm)
 Definition value_ind' (P : value -> Prop)
     (HConstr :  forall tag args, Forall P args -> P (Constr tag args))
     (HClose :   forall fname free, Forall P free -> P (Close fname free))
+    (HOpaque :  forall ty v, P (Opaque ty v))
     (v : value) : P v :=
     ltac:(refine (@value_rect_mut P (Forall P)
-        HConstr HClose _ _ v); eauto).
+        HConstr HClose HOpaque _ _ v); eauto).
 
 
 Inductive public_value (M : list metadata) : value -> Prop :=
@@ -76,7 +85,8 @@ Inductive public_value (M : list metadata) : value -> Prop :=
         m_access m = Public ->
         Forall (public_value M) free ->
         length free = m_nfree m ->
-        public_value M (Close fname free).
+        public_value M (Close fname free)
+| PvOpaque : forall ty v, public_value M (Opaque ty v).
 
 
 Definition value_eq_dec (x y : value) : { x = y } + { x <> y }.
@@ -94,6 +104,13 @@ induction x using value_rect_mut with
   destruct (IHx free0); [ | right; congruence ]. subst free0.
   left. reflexivity.
 
+- destruct y; try solve [right; inversion 1].
+  destruct (opaque_type_name_eq_dec ty ty0); [ | right; congruence ]. subst ty0.
+  destruct (opaque_type_denote_eq_dec _ v v0); cycle 1.
+    { right. inversion 1. fix_existT. congruence. }
+    subst v0.
+  left. reflexivity.
+
 - destruct ys; try solve [right; inversion 1].
   left. reflexivity.
 
@@ -102,3 +119,170 @@ induction x using value_rect_mut with
   destruct (IHx0 ys); [ | right; congruence ]. subst ys.
   left. reflexivity.
 Defined.
+
+
+
+Definition VForall (P : value -> Prop) : value -> Prop :=
+    let fix go v :=
+        let fix go_list vs :=
+            match vs with
+            | [] => True
+            | v :: vs => go v /\ go_list vs
+            end in
+        P v /\
+        match v with
+        | Constr _ args => go_list args
+        | Close _ free => go_list free
+        | Opaque _ _ => True
+        end in go.
+
+Definition VForall_list (P : value -> Prop) :=
+    let go := VForall P in
+    let fix go_list vs :=
+        match vs with
+        | [] => True
+        | v :: vs => go v /\ go_list vs
+        end in go_list.
+
+Ltac refold_VForall P := fold (VForall_list P) in *.
+
+Lemma VForall_this : forall P v, VForall P v -> P v.
+destruct v; inversion 1; eauto.
+Qed.
+
+
+
+Definition VExists (P : value -> Prop) : value -> Prop :=
+    let fix go v :=
+        let fix go_list vs :=
+            match vs with
+            | [] => False
+            | v :: vs => go v \/ go_list vs
+            end in
+        P v \/
+        match v with
+        | Constr _ args => go_list args
+        | Close _ free => go_list free
+        | Opaque _ _ => False
+        end in go.
+
+Definition VExists_list (P : value -> Prop) :=
+    let go := VExists P in
+    let fix go_list vs :=
+        match vs with
+        | [] => True
+        | v :: vs => go v /\ go_list vs
+        end in go_list.
+
+Ltac refold_VExists P := fold (VExists_list P) in *.
+
+Lemma VExists_this : forall (P : value -> Prop) v, P v -> VExists P v.
+intros. destruct v; left; eauto.
+Qed.
+
+
+
+Definition VIn (v0 : value) : value -> Prop :=
+    let fix go v :=
+        let fix go_list vs :=
+            match vs with
+            | [] => False
+            | v :: vs => go v \/ go_list vs
+            end in
+        v0 = v \/
+        match v with
+        | Constr _ args => go_list args
+        | Close _ free => go_list free
+        | Opaque _ _ => False
+        end in go.
+
+Definition VIn_list v0 :=
+    let go := VIn v0 in
+    let fix go_list vs :=
+        match vs with
+        | [] => False
+        | v :: vs => go v \/ go_list vs
+        end in go_list.
+
+Lemma unroll_VIn : forall v0 v,
+    VIn v0 v = (
+        v0 = v \/
+        match v with
+        | Constr _ args => VIn_list v0 args
+        | Close _ free => VIn_list v0 free
+        | Opaque _ _ => False
+        end).
+destruct v; simpl; fold (VIn_list v0) in *; reflexivity.
+Qed.
+
+Lemma unroll_VIn_list : forall v0 vs,
+    VIn_list v0 vs = (
+        match vs with
+        | [] => False
+        | v :: vs => VIn v0 v \/ VIn_list v0 vs
+        end).
+destruct vs; simpl; fold (VIn_list v0) in *; reflexivity.
+Qed.
+
+Opaque VIn.
+Opaque VIn_list.
+
+Lemma VIn_this : forall v, VIn v v.
+intros. destruct v; left; eauto.
+Qed.
+
+
+Lemma VForall_VIn : forall P v,
+    VForall P v <-> (forall v', VIn v' v -> P v').
+intro P.
+induction v using value_rect_mut with
+    (Pl := fun vs =>
+        VForall_list P vs <-> (forall v', VIn_list v' vs -> P v'));
+simpl; refold_VForall P.
+
+- split; intro HH; intros.
+  + break_and. rewrite unroll_VIn in *. break_or; try congruence.
+    eapply IHv; eauto.
+  + split.
+    -- eapply HH. rewrite unroll_VIn. eauto.
+    -- rewrite IHv. intros. eapply HH. rewrite unroll_VIn. eauto.
+
+- split; intro HH; intros.
+  + break_and. rewrite unroll_VIn in *. break_or; try congruence.
+    eapply IHv; eauto.
+  + split.
+    -- eapply HH. rewrite unroll_VIn. eauto.
+    -- rewrite IHv. intros. eapply HH. rewrite unroll_VIn. eauto.
+
+- split; intro HH; intros.
+  + rewrite unroll_VIn in *. break_or; try contradiction.
+    break_and. congruence.
+  + split; eauto. eapply HH. eapply VIn_this.
+
+
+- split; eauto. intros.
+  rewrite unroll_VIn_list in *. contradiction.
+
+- split; intro HH; intros.
+  + rewrite unroll_VIn_list in *. break_and. break_or.
+    -- eapply IHv; eauto.
+    -- eapply IHv0; eauto.
+  + split.
+    -- rewrite IHv. intros. eapply HH. rewrite unroll_VIn_list. eauto.
+    -- rewrite IHv0. intros. eapply HH. rewrite unroll_VIn_list. eauto.
+Qed.
+
+Lemma VForall_VIn_list : forall P vs,
+    VForall_list P vs <-> (forall v', VIn_list v' vs -> P v').
+induction vs; split; intro HH; intros.
+- rewrite unroll_VIn_list in *. contradiction.
+- constructor.
+- simpl in *. refold_VForall P. break_and.
+  rewrite unroll_VIn_list in *. break_or.
+  + on _, rewrite_fwd VForall_VIn. eauto.
+  + on _, rewrite_fwd IHvs. eauto.
+- simpl. refold_VForall P. split.
+  + rewrite VForall_VIn. intros. eapply HH. rewrite unroll_VIn_list. eauto.
+  + rewrite IHvs. intros. eapply HH. rewrite unroll_VIn_list. eauto.
+Qed.
+
